Current state commented out with Glob_term

Monad.v
@@ -1,1 +1,21 @@
 Declare ML Module "monadPlugin".
+
+Set Implicit Arguments.
+
+Class Monad (t : Type -> Type) : Type := {
+  ret : forall A, A -> t A;
+  bind : forall A B, t A -> (A -> t B) -> t B}.
+
+Module State.
+  Definition t (S : Type) : Type -> Type :=
+    fun A => S -> A * S.
+  
+  Instance Monad (S : Type) : Monad (t S) := {
+    ret := fun _ x =>
+      fun s => (x, s);
+    bind := fun _ _ x f =>
+      fun s =>
+        let (x', s') := x s in
+        f x' s'}.
+End State.
+
