tests/1.v
@@ -1,6 +1,16 @@
 Require Import Monad.
 
-Monadic f := 12.
-Check f.
+Set Implicit Arguments.
+
+Definition M := State.t bool.
+
+Definition incr (n : nat) : M nat :=
+  ret (n + 1).
+
+Definition twelve : M nat :=
+  ret 12.
+
+Monadic f := (incr (incr twelve)).
+Print f.
 
 
