src/monad.ml4
@@ -1,8 +1,27 @@
+(*let unfold_apps f xs : Glob_term.glob_constr =
+  List.fold_left (fun f x -> Glob_term.GApp (Loc.ghost, f, [ x ])) f xs
 
+let rec monadise (e : Glob_term.glob_constr) : Constr.t =
+  match e with
+  | Glob_term.GApp (loc, f, xs) ->
+    if List.length xs <> 1 then
+      monadise (unfold_apps f xs)
+    else
+      let f = monadise f in
+      let x = monadise (List.hd xs) in
+      let type_of = Typing.type_of (Global.env ()) Evd.empty in
+      (match Typeclasses.class_of_constr (type_of x) with
+      | None -> Constr.mkApp (f, [|x|])
+      | Some _ -> failwith "TODO")
+  | _ -> e*)
 
 (** Syntax extension do add a "Monadic" command to define new monadic terms. *)
 VERNAC COMMAND EXTEND Monadic CLASSIFIED AS SIDEFF
 | [ "Monadic" ident(name) ":=" constr(value) ] -> [
+  (*Pp.msg_info (Pp.str "1");
+  let value = Constrintern.intern_constr Evd.empty (Global.env ()) value in
+  failwith "gre";
+  let value = monadise value in*)
   let value = Constrintern.interp_constr Evd.empty (Global.env ()) value in
   let _ = Declare.declare_definition name (Future.from_val (value, Declareops.no_seff)) in
   () ]
